\documentclass[11pt]{article}

\usepackage[margin=2cm]{geometry}

\title{Mathematics Literacy Basic Arithmetic Practise Questions}

\begin{document}
\maketitle

\section{Arithmetic}

\subsection{Addition}
\begin{enumerate}
	\item ${{ addition[0] }} + {{ addition[1] }} =$
	\item ${{ addition[2] }} + {{ addition[3] }} =$
	\item ${{ addition[4] }} + {{ addition[5] }} =$
	\item ${{ addition[6] }} + {{ addition[7] }} =$
	\item ${{ addition[8] }} + {{ addition[9] }} + {{ addition[10] }} =$
	\item ${{ addition[11] }} + {{ addition[12] }} =$
	\item ${{ addition[13] }} + {{ addition[14] }} + {{ addition[15] }} =$
	\item ${{ addition[16] }} + {{ addition[17] }} + {{ addition[18] }} =$
	\item ${{ addition[19] }} + {{ addition[20] }} + {{ addition[21] }} =$
	\item ${{ addition[22] }} + {{ addition[23] }} =$
	\item ${{ addition[24] }} + {{ addition[25] }} =$
	\item ${{ addition[26] }} + {{ addition[27] }} + {{ addition[28] }} =$
	\item ${{ addition[29] }} + {{ addition[30] }} =$
	\item ${{ addition[31] }} + {{ addition[32] }} =$
	\item ${{ addition[33] }} + {{ addition[34] }} + {{ addition[35] }} =$
	\item ${{ addition[36] }} + {{ addition[37] }} + {{ addition[38] }} =$
	\item ${{ addition[39] }} + {{ addition[40] }} =$
	\item ${{ addition[41] }} + {{ addition[42] }} =$
\end{enumerate}

\clearpage

\subsection{Subtraction}
\begin{enumerate}
	\item ${{ subtraction[0] }} - {{ subtraction[1] }} =$
	\item ${{ subtraction[2] }} - {{ subtraction[3] }} =$
	\item ${{ subtraction[4] }} - {{ subtraction[5] }} =$
	\item ${{ subtraction[6] }} - {{ subtraction[7] }} =$
	\item ${{ subtraction[8] }} - {{ subtraction[9] }} - {{ subtraction[10] }} =$
	\item ${{ subtraction[11] }} - {{ subtraction[12] }} =$
	\item ${{ subtraction[13] }} - {{ subtraction[14] }} - {{ subtraction[15] }} =$
	\item ${{ subtraction[16] }} - {{ subtraction[17] }} - {{ subtraction[18] }} =$
	\item ${{ subtraction[19] }} - {{ subtraction[20] }} - {{ subtraction[21] }} =$
	\item ${{ subtraction[22] }} - {{ subtraction[23] }} =$
	\item ${{ subtraction[24] }} - {{ subtraction[25] }} =$
	\item ${{ subtraction[26] }} - {{ subtraction[27] }} - {{ subtraction[28] }} =$
	\item ${{ subtraction[29] }} - {{ subtraction[30] }} =$
	\item ${{ subtraction[31] }} - {{ subtraction[32] }} =$
	\item ${{ subtraction[33] }} - {{ subtraction[34] }} - {{ subtraction[35] }} =$
	\item ${{ subtraction[36] }} - {{ subtraction[37] }} - {{ subtraction[38] }} =$
	\item ${{ subtraction[39] }} - {{ subtraction[40] }} =$
	\item ${{ subtraction[41] }} - {{ subtraction[42] }} =$
\end{enumerate}

\end{document}
